Generalize wordcount thm to the same form as on the ISA level

hardware/ag32StepLib.sml
@@ -1,0 +1,30 @@
+structure ag32StepLib =
+struct
+
+open hardwarePreamble;
+
+open ag32MachineTheory;
+
+(* Memory behavior-selection functions *)
+
+local
+  val is_mem_def = ``is_mem fext_accessor_circuit step' fext``
+  |> SIMP_CONV (srw_ss()) [fext_accessor_circuit_def, is_mem_def]
+  |> GEN_ALL;
+  fun rw_mem conjn n = el conjn o CONJUNCTS o Q.SPEC n o PURE_REWRITE_RULE [is_mem_def]
+in
+val is_mem_do_nothing = rw_mem 1
+val is_mem_inst_read = rw_mem 2
+val is_mem_data_read = rw_mem 3
+val is_mem_data_write = rw_mem 4
+val is_mem_data_flush = rw_mem 5
+(* special: *)
+val is_mem_def_mem_no_errors = el 6 o CONJUNCTS o SPEC_ALL o PURE_REWRITE_RULE [is_mem_def]
+end
+
+(* Can be optimized ... *)
+val no_mem_error_tac = reverse IF_CASES_TAC
+                       >- rfs [is_mem_def, mem_no_errors_def] \\
+                       pop_assum kall_tac;
+
+end
