cakeml_connection/wordcountVerilogProofScript.sml
@@ -3,7 +3,7 @@ open hardwarePreamble;
 open wordcountProofTheory;
 
 open verilogTypeTheory moduleTranslatorTheory;
-open ag32MachineTheory ag32EqTheory ag32VerilogTheory;
+open ag32MachineTheory ag32EqTheory ag32HaltTheory ag32VerilogTheory;
 
 open commonVerilogProofTheory;
 
@@ -12,21 +12,25 @@ val _ = new_theory "wordcountVerilogProof";
 val _ = guess_lengths ();
 val _ = prefer_num ();
 
+val get_mem_word_word_at_addr = Q.store_thm("get_mem_word_word_at_addr",
+ `!mem addr. get_mem_word mem addr = word_at_addr mem addr`,
+ rw [word_at_addr_def, ag32_memoryTheory.get_mem_word_def]);
+
 val wordcount_ag32_next_verilog = Q.store_thm("wordcount_ag32_next_verilog",
- `!vstep fext fextv init cl inp.
+ `!vstep fext fextv init inp.
    vars_has_type init ag32_verilog_types ∧
    INIT_verilog (fext 0) init ∧
 
    vstep = mrun fextv computer init ∧
 
    is_lab_env fext_accessor_verilog vstep fext ∧
-   (fext 0).mem = (wordcount_init_memory ([strlit "wordcount"], inp)) ∧
+   (fext 0).mem = (init_memory code data (THE config.ffi_names) ([strlit "wordcount"], inp)) ∧
    lift_fext fextv fext ∧
 
    STRLEN inp ≤ stdin_size
    ⇒
-   ?k fin.
-    vstep k = INR fin /\
+   ?k1. !k. k1 ≤ k ==>
+    ?fin. vstep k = INR fin /\
     let outs = MAP get_ag32_io_event (fext k).io_events;
         outs_spec = MAP get_output_io_event (wordcount_io_events inp) in
       ag32_is_halted fin wordcount_machine_config ∧
@@ -51,12 +55,63 @@ val wordcount_ag32_next_verilog = Q.store_thm("wordcount_ag32_next_verilog",
 
  drule_strip (SIMP_RULE (srw_ss()) [] INIT_REL_circuit_verilog) \\
  pop_assum(qspec_then`k1`strip_assume_tac) \\
- asm_exists_tac \\
- fs [REL_def, ag32_is_halted_def, wordcount_machine_config_def,
-     ag32_machine_configTheory.ag32_machine_config_def] \\ conj_tac
+ qexists_tac `m` \\ rpt strip_tac' \\
+
+ fs [is_lab_env_def] \\
+ drule_strip is_mem_verilog \\
+ drule_strip is_interrupt_interface_verilog \\
+ drule_strip (SIMP_RULE (srw_ss()) [] circuit_halt_compute_step_full_actual') \\
+ fs [arithmeticTheory.LESS_EQ_EXISTS] \\ rveq \\
+ disch_then (qspecl_then [`m`, `p'`] mp_tac) \\ impl_tac
+ >- (rpt conj_tac
+    >- (fs [REL_def] \\ EVAL_TAC \\ simp [wordcountCompileTheory.config_def])
+    >- rfs [REL_def, get_mem_word_word_at_addr]
+    >- fs [halt_inv_def, REL_def]) \\
+ strip_tac \\
+
+ drule_strip computer_Next_relM_run \\ pop_assum (qspec_then `p' + m` strip_assume_tac) \\
+ fs [REL_def, ag32_is_halted_def, ag32_machine_configTheory.ag32_machine_config_def] \\ conj_tac
 
  >- fs [relM_def, relM_var_def, WORD_def]
 
- \\ strip_tac \\ drule_strip after_R_lift \\ drule_first);
+ \\ strip_tac \\ rfs [] \\ drule_strip after_R_1w_lift \\ drule_first);
+
+val is_prefix_extract_writes = Q.store_thm("is_prefix_extract_writes",
+ `!l1 l2 fd. l1 ≼ l2 ==> extract_writes fd l1 ≼ extract_writes fd l2`,
+ Induct >- rw [ag32_basis_ffiProofTheory.extract_writes_def] \\
+
+ rw [] \\ every_case_tac \\ fs [] \\
+ rveq \\ first_x_assum drule \\ disch_then (qspec_then `fd` assume_tac) \\
+ fs [ag32_basis_ffiProofTheory.extract_writes_def] \\ rw []);
+
+val wordcount_ag32_next_verilog_prettier = Q.store_thm("wordcount_ag32_next_verilog_prettier",
+ `!vstep fext fextv init inp.
+   vars_has_type init ag32_verilog_types ∧
+   INIT_verilog (fext 0) init ∧
+
+   vstep = mrun fextv computer init ∧
+
+   is_lab_env fext_accessor_verilog vstep fext ∧
+   (fext 0).mem = (init_memory code data (THE config.ffi_names) ([strlit "wordcount"], inp)) ∧
+   lift_fext fextv fext ∧
+
+   STRLEN inp ≤ stdin_size
+   ⇒
+   ?k1.
+    !k. k1 ≤ k ==>
+    ?fin. vstep k = INR fin /\
+    let outs = MAP get_ag32_io_event (fext k).io_events;
+        outs_stdout = extract_writes 1 outs;
+        outs_stdout_spec = explode (concat
+                             [toString (LENGTH (TOKENS isSpace inp)); strlit " ";
+                              toString (LENGTH (splitlines inp)); strlit "\n"])
+    in
+      ag32_is_halted fin wordcount_machine_config ∧
+      outs_stdout ≼ outs_stdout_spec ∧
+      (exit_code_0 fin (fextv k) ⇒
+       outs_stdout = outs_stdout_spec)`,
+ metis_tac [wordcount_ag32_next_verilog,
+            wordcount_extract_writes_stdout,
+            is_prefix_extract_writes]);
 
 val _ = export_theory ();
