hardware/ag32HaltScript.sml
@@ -1,0 +1,225 @@
+open hardwarePreamble;
+
+open ag32MachineTheory ag32EqTheory;
+
+open ag32StepLib;
+
+val _ = new_theory "ag32Halt";
+
+val _ = guess_lengths ();
+val _ = prefer_num ();
+
+(* This file is thrown together and should not depend on ag32EqTheory *)
+
+val Encode_Jump_decode_instruction = Q.store_thm("Encode_Jump_decode_instruction",
+ `!s. s.i = Encode (Jump (fAdd,0w,Imm 0w)) ==> decode_instruction s = s with instruction := 9w`,
+ rw [ag32Theory.Encode_def, ag32Theory.enc_def, ag32Theory.ri2bits_def] \\
+ rw [decode_instruction_def]);
+
+val circuit_halt_compute_step = Q.store_thm("circuit_halt_compute_step",
+`!n c init fext facc.
+ c = circuit facc init fext /\
+ is_mem fext_accessor_circuit c fext /\
+ is_interrupt_interface fext_accessor_circuit c fext /\
+ (c n).state = 0w /\
+ (c n).i = word_at_addr (fext n).mem ((c n).PC) /\
+ (c n).command = 0w /\
+ ~(c n).interrupt_req /\
+ (fext n).ready /\
+ (fext n).interrupt_state = InterruptReady /\
+ (word_at_addr (fext n).mem (c n).PC = Encode (Jump (fAdd, 0w, Imm 0w)))
+ ==>
+ ?carryflag overflowflag.
+ (fext (n + 1)).mem = (fext n).mem ∧
+ (fext (n + 1)).ready = (fext n).ready ∧
+ (fext (n + 1)).interrupt_state = InterruptReady /\
+ (fext (n + 1)).io_events = (fext n).io_events ∧
+ cpu_eq (c (n + 1))
+        (c n with
+           <|state := 1w; R := (0w =+ (c n).PC + 4w) (c n).R;
+             CarryFlag := carryflag; OverflowFlag := overflowflag;
+             command := 1w|>)`,
+ rpt strip_tac \\ rveq \\
+
+ (* mem *)
+ last_assum (assume_tac o is_mem_do_nothing `n`) \\
+ fs [arithmeticTheory.ADD1] \\
+ pop_assum kall_tac \\
+
+ (* interrupt *)
+ drule_strip no_interrupt_req \\ fs [arithmeticTheory.ADD1] \\
+
+ simp [GSYM arithmeticTheory.ADD1, circuit_def, cpu_Next_def] \\
+ no_mem_error_tac \\
+ simp [cpu_Next_0w_def, Encode_Jump_decode_instruction, DecodeReg_imm_def] \\
+
+ fs [ag32Theory.Encode_def, ag32Theory.enc_def, ag32Theory.ri2bits_def] \\
+ simp [ALU_def, execute_instruction_def] \\
+
+ rw [cpu_eq_def] \\ blastLib.BBLAST_TAC);
+
+val circuit_halt_compute_step2_SUC = Q.store_thm("circuit_halt_compute_step2_SUC",
+`!n c init fext facc.
+ c = circuit facc init fext /\
+ mem_no_errors fext /\
+ (c n).state = 1w /\
+ (c n).command = 0w /\
+ (c n).do_delay_write = 5w /\
+ ~(c n).do_interrupt /\
+ ~(c n).interrupt_req /\
+ (fext n).ready /\
+ (fext n).interrupt_state = InterruptReady ==>
+ cpu_eq (c (SUC n)) ((c n) with <| state := 0w; i := (fext n).inst_rdata |>)`,
+ rw [circuit_def] \\ simp [cpu_Next_def] \\ no_mem_error_tac \\
+ simp [cpu_Next_1w_def, delay_write_Next_def, cpu_eq_def]);
+
+val circuit_halt_compute_step2 = Q.store_thm("circuit_halt_compute_step2",
+`!n c init fext facc s.
+ c = circuit facc init fext /\
+ is_mem fext_accessor_circuit c fext /\
+ is_interrupt_interface fext_accessor_circuit c fext /\
+ (c n).state = 1w /\
+ (c n).command = 1w /\
+ (c n).do_delay_write = 5w /\
+ ~(c n).do_interrupt /\
+ ~(c n).interrupt_req /\
+ (fext n).ready /\
+ (fext n).interrupt_state = InterruptReady
+ ==>
+ ?m. (fext (n + m)).mem = (fext n).mem ∧
+     (fext (n + m)).ready = (fext n).ready ∧
+     (fext (n + m)).interrupt_state = InterruptReady /\
+     (!l. l <= m ==> (fext (n + l)).io_events = (fext n).io_events /\
+                     (c (n + l)).R = (c n).R /\
+                     (c (n + l)).PC = (c n).PC) /\
+     cpu_eq (c (n + m))
+            (c n with
+               <|command := 0w;
+                 state := 0w;
+                 i := word_at_addr (fext n).mem (align_addr (c n).PC) |>)`,
+ (* copied from circuit_next more or less, should make more modular thms instead... *)
+ rpt strip_tac' \\ last_assum (mp_tac o is_mem_inst_read `n`) \\
+ simp [] \\ strip_tac \\
+ drule_strip is_mem_mem_no_errors \\
+ drule_strip circuit_read_wait \\ simp [] \\ strip_tac \\
+ qpat_x_assum `cpu_eq _ _` (strip_assume_tac o REWRITE_RULE [cpu_eq_def]) \\ rfs [] \\
+
+ qexists_tac `m + 2` \\ once_rewrite_tac [DECIDE ``m + 2 + n = SUC (SUC (m + n))``] \\
+
+ drule_strip (SIMP_RULE (srw_ss()) [] circuit_halt_compute_step2_SUC) \\
+ pop_assum (strip_assume_tac o REWRITE_RULE [cpu_eq_def]) \\ rfs [] \\
+
+ last_assum (mp_tac o is_mem_do_nothing `SUC (m + n)`) \\
+ impl_tac >- simp [] \\ strip_tac \\
+ drule_strip no_interrupt_req \\ simp [cpu_eq_def] \\
+
+ rpt strip_tac' \\ `l <= SUC m \/ l = m + 2` by decide_tac \\
+ fs [arithmeticTheory.ADD1] \\ first_x_assum (qspec_then `SUC m` mp_tac) \\ 
+ simp [arithmeticTheory.ADD1]);
+
+val halt_inv_def = Define `
+ halt_inv c fext n <=>
+  (c n).i = word_at_addr (fext n).mem (align_addr (c n).PC) /\
+  (c n).state = 0w /\
+  (c n).command = 0w /\
+  ~(c n).interrupt_req /\
+  (fext n).ready /\
+  (fext n).interrupt_state = InterruptReady /\
+  (c n).do_delay_write = 5w ∧
+  ¬(c n).do_interrupt`;
+
+val byte_aligned_align_addr = Q.store_thm("byte_aligned_align_addr",
+ `!(w:word32). byte_aligned w ==> align_addr w = w`,
+ rw [alignmentTheory.byte_aligned_def, alignmentTheory.aligned_def,
+     alignmentTheory.align_def, align_addr_def] \\
+ blastLib.FULL_BBLAST_TAC);
+
+val circuit_halt_compute_step_full = Q.store_thm("circuit_halt_compute_step_full",
+ `!n c init fext facc s.
+   c = circuit facc init fext /\
+   is_mem fext_accessor_circuit c fext /\
+   is_interrupt_interface fext_accessor_circuit c fext /\
+   halt_inv c fext n /\
+   byte_aligned (c n).PC /\
+   word_at_addr (fext n).mem (c n).PC = Encode (Jump (fAdd,0w,Imm 0w))
+   ==>
+   ?m. halt_inv c fext (SUC (n + m)) /\
+       (fext (SUC (n + m))).mem = (fext n).mem /\
+       (fext (SUC (n + m))).ready = (fext n).ready /\
+       (c (SUC (n + m))).PC = (c n).PC /\
+       (!l. l <= SUC m ==> (fext (n + l)).io_events = (fext n).io_events /\
+                           (c (n + l)).R 1w = (c n).R 1w /\
+                           (c (n + l)).PC = (c n).PC)`,
+ rpt strip_tac \\
+ qpat_x_assum `halt_inv _ _ _` (STRIP_ASSUME_TAC o REWRITE_RULE [halt_inv_def]) \\
+
+ rveq \\
+ drule_strip (SIMP_RULE (srw_ss()) [] circuit_halt_compute_step2) \\
+ disch_then (qspec_then `n + 1` mp_tac) \\
+
+ drule_strip (SIMP_RULE (srw_ss()) [] circuit_halt_compute_step) \\
+
+ qpat_abbrev_tac `c = circuit _ _ _` \\
+
+ simp [byte_aligned_align_addr] \\
+ disch_then (STRIP_ASSUME_TAC o SIMP_RULE (srw_ss()) [cpu_eq_def]) \\
+
+ simp [] \\
+ strip_tac \\
+
+ qexists_tac `m` \\ fs [halt_inv_def, cpu_eq_def, arithmeticTheory.ADD1,
+                        combinTheory.APPLY_UPDATE_THM] \\
+ rpt strip_tac' \\ `l = 0 \/ (0 < l /\ l <= m) \/ l = m + 1` by decide_tac \\ fs []
+ >- (first_x_assum (qspec_then `l - 1` mp_tac) \\ simp [combinTheory.APPLY_UPDATE_THM])
+ >- simp [combinTheory.APPLY_UPDATE_THM]);
+
+val circuit_halt_compute_step_full_actual = Q.store_thm("circuit_halt_compute_step_full_actual",
+ `!n m c init fext facc s.
+   c = circuit facc init fext /\
+   is_mem fext_accessor_circuit c fext /\
+   is_interrupt_interface fext_accessor_circuit c fext /\
+   byte_aligned (c n).PC /\
+   word_at_addr (fext n).mem (c n).PC = Encode (Jump (fAdd,0w,Imm 0w)) /\
+   halt_inv c fext n
+   ==>
+   ?l. m <= l /\
+       halt_inv c fext (n + l) /\
+       (fext (n + l)).mem = (fext n).mem ∧
+       (c (n + l)).PC = (c n).PC ∧
+       (!k. k <= l ==> (fext (n + k)).io_events = (fext n).io_events /\
+                       (c (n + k)).R 1w = (c n).R 1w /\
+                       (c (n + k)).PC = (c n).PC)`,
+ rpt strip_tac \\ rveq \\ Induct_on `m` \\ rpt strip_tac >- (qexists_tac `0` \\ rw []) \\
+
+ pop_assum strip_assume_tac \\
+ drule_strip (SIMP_RULE (srw_ss()) [] circuit_halt_compute_step_full) \\
+ impl_tac >- simp [] \\ strip_tac \\
+
+ qexists_tac `l + m' + 1` \\ fs [arithmeticTheory.ADD1] \\
+ rpt strip_tac' \\ 
+ last_assum (qspec_then `l` mp_tac) \\ impl_tac >- simp [] \\ strip_tac \\
+ fs [] \\
+
+ Cases_on `k ≤ l`
+ >- metis_tac []
+ \\ fs []
+ \\ `l ≤ k` by decide_tac
+ \\ ntac 2 (first_x_assum (qspec_then `k - l` mp_tac))
+ \\ simp []);
+
+val circuit_halt_compute_step_full_actual' = Q.store_thm("circuit_halt_compute_step_full_actual'",
+ `!n m c init fext facc s.
+   c = circuit facc init fext /\
+   is_mem fext_accessor_circuit c fext /\
+   is_interrupt_interface fext_accessor_circuit c fext /\
+   byte_aligned (c n).PC /\
+   word_at_addr (fext n).mem (c n).PC = Encode (Jump (fAdd,0w,Imm 0w)) /\
+   halt_inv c fext n
+   ==>
+   (c (n + m)).PC = (c n).PC /\
+   (fext (n + m)).io_events = (fext n).io_events /\
+   (c (n + m)).R 1w = (c n).R 1w`,
+ metis_tac [circuit_halt_compute_step_full_actual]);
+
+val _ = export_theory ();
+
